ObsTrace.v
@@ -1,0 +1,274 @@
+Require Import Trace.
+
+Variable Word:Type.
+
+(* Observations are values, or silent (tau) *)
+Inductive Observation :=
+| Out (w : Word)
+| Tau.
+
+Definition ObsTrace := TraceOf Observation.
+
+Ltac app_frobber :=
+  repeat match goal with
+         | |- context[(finished ?T) ^ ?OT] =>
+           rewrite (idTrace_eq (finished T ^ OT)); simpl
+         | |- context[(notfinished ?O ?T) ^ ?OT] =>
+           rewrite (idTrace_eq (notfinished O T ^ OT)); simpl
+         | [H: context[(finished ?T) ^ ?OT] |- _ ] =>
+           rewrite (idTrace_eq (finished T ^ OT)) in H; simpl in H
+         | [H: context[(notfinished ?O ?T) ^ ?OT] |- _ ] =>
+           rewrite (idTrace_eq (notfinished O T ^ OT)) in H; simpl in H
+         end.
+
+(********************** ObsTrace Equivalence *************************)
+
+CoInductive ObsTraceEq : TraceOf Observation -> TraceOf Observation -> Prop :=
+| ObsEqTau1 : forall OO OO',
+    ObsTraceEq OO OO' ->
+    ObsTraceEq (notfinished Tau OO) OO'
+| ObsEqTau2 : forall OO OO',
+    ObsTraceEq OO OO' ->
+    ObsTraceEq OO (notfinished Tau OO')
+| ObsEqNow : forall w OO OO',
+    ObsTraceEq OO OO' ->
+    ObsTraceEq (notfinished (Out w) OO) (notfinished (Out w) OO')
+| ObsEqFinishedOut : forall w,
+    ObsTraceEq (finished (Out w)) (finished (Out w))
+| ObsEqFinishedTau :
+    ObsTraceEq (finished Tau) (finished Tau)
+(* The last thing we need is a way of handling *all-tau* traces.
+   There are a couple of ways of doing that, not sure what will
+   play better in proofs. *)
+| ObsEqAllTau : forall OO,
+     ObsTraceEq OO OO.
+(* APT: Establishing equality between traces seems hard, and this overlaps
+the previous two cases.  Maybe try:
+   ForallTrace (fun o => o = Tau) OO ->
+   ForallTrace (fun o => o = Tau) OO' ->
+   ObsTraceEq OO OO'
+?
+LEO: That was the other thing I had in mind. I'll see what makes proofs easier.
+(Note that this proposal overlaps with the first two cases, as well as the last one.)
+ *)
+
+Lemma ObsTraceEq_sym :
+  forall O O',
+    ObsTraceEq O O' -> ObsTraceEq O' O.
+Proof.
+  cofix COFIX. 
+  intros.
+  inversion H; subst; clear H;
+    try (constructor; apply COFIX; auto). 
+Qed.
+
+Lemma ObsTraceEqRemoveTau1 :
+  forall T T', ObsTraceEq (notfinished Tau T) T' -> ObsTraceEq T T'.
+Proof.
+  cofix COFIX.
+  intros T T' Eq.
+  inversion Eq; subst; clear Eq.
+  + auto.
+  + eapply ObsEqTau2.
+    eapply COFIX; auto.
+  + eapply ObsEqTau2.
+    eapply ObsEqAllTau.
+Qed.
+
+Lemma ObsTraceEqRemoveTau2 :
+  forall T T', ObsTraceEq T (notfinished Tau T') -> ObsTraceEq T T'.
+Proof.
+  cofix COFIX.
+  intros T T' Eq.
+  inversion Eq; subst; clear Eq.
+  + eapply ObsEqTau1.
+    eapply COFIX.
+    auto.
+  + auto. 
+  + eapply ObsEqTau1.
+    eapply ObsEqAllTau.
+Qed.
+
+Fixpoint tauN (n : nat) (T : TraceOf Observation) : TraceOf Observation :=
+  match n with
+  | O => T
+  | S n' => notfinished Tau (tauN n' T)
+  end.
+
+Lemma EqOut_tauN : forall T' t',
+    Last T' t' ->
+    forall w T, 
+      ObsTraceEq (notfinished (Out w) T) T' ->
+      exists n, T' = tauN n (finished (Out w)) \/ exists  T'', T' = tauN n (notfinished (Out w) T'').
+Proof.
+  intros T' t' HL.
+  induction HL; intros w Tw Eq.
+  - exists 0. left. simpl.
+    inversion Eq.
+  - destruct a'.
+    + inversion Eq; subst; clear Eq.
+      * exists 0.
+        right.
+        exists T; simpl; auto.
+      * exists 0.
+        right.
+        exists T; simpl; auto.
+    + inversion Eq; subst; clear Eq.
+      destruct (IHHL w Tw H1) as [n [HTau | [T'' HTau]]].
+      * exists (S n).
+        left.
+        simpl.
+        rewrite HTau.
+        auto.
+      * exists (S n).
+        right.
+        simpl.
+        exists T''.
+        rewrite HTau.
+        auto.
+Qed.
+
+Lemma ObsTraceEqApp :
+  forall O1 O1' O2 O2' o1 o1',
+    Last O1 o1 -> Last O1' o1' -> 
+    ObsTraceEq O1 O1' ->
+    ObsTraceEq O2 O2' ->
+    ObsTraceEq (O1^(Some O2)) (O1'^(Some O2')).
+Proof.
+    intros O1 O1' O2 O2' o1 o1' H;
+    revert O1' O2 O2' o1'.
+  induction H as [o1|]; intros O1' O2 O2' o1' Last' Eq1 Eq2.
+  - generalize dependent O2;
+    generalize dependent O2';
+    generalize dependent Eq1.
+    induction Last';
+      intros Eq1 O2' O2 Eq2.
+    + inversion Eq1; subst; simpl in *; clear Eq1; app_frobber.
+      * apply ObsEqNow; auto.
+      * apply ObsEqTau1; apply ObsEqTau2; auto.
+      * destruct a.
+        -- apply ObsEqNow; auto.
+        -- apply ObsEqTau1; apply ObsEqTau2; auto.
+    + inversion Eq1; subst; simpl in *; clear Eq1.
+      specialize (IHLast' H1 O2' O2 Eq2).      
+      app_frobber.
+      eapply ObsEqTau2.
+      auto.
+  - destruct a'.
+    + destruct (EqOut_tauN O1' o1' Last' w T Eq1) as [n [HTau | [T' HTau]]].
+      * rewrite HTau in *.
+        clear HTau.
+        induction n; simpl in *; subst; app_frobber.
+        -- apply ObsEqNow.
+           inversion Eq1.
+        -- apply ObsEqTau2.
+           inversion Last'; subst; clear Last'.
+           apply ObsTraceEqRemoveTau2 in Eq1.
+           specialize (IHn H3 Eq1).
+           auto.
+      * rewrite HTau in *.
+        clear HTau.
+        induction n; simpl in *; subst; app_frobber.
+        -- apply ObsEqNow.
+           inversion Eq1; subst; clear Eq1.
+           ++ inversion Last'; subst; clear Last'.
+              eauto.
+           ++ inversion Last'; subst; clear Last'.
+              eauto using ObsEqAllTau.
+        -- inversion Last'; subst; clear Last'.
+           specialize (IHn H3).
+           apply ObsTraceEqRemoveTau2 in Eq1.
+           specialize (IHn Eq1).
+           apply ObsEqTau2.
+           auto.
+    + apply ObsTraceEqRemoveTau1 in Eq1.
+      app_frobber.
+      apply ObsEqTau1.
+      eauto.
+Qed.
+
+(********************** ObsTrace Prefix *************************)
+
+(* The second is a prefix of the first, up to Tau *)
+CoInductive ObsTracePrefix : TraceOf Observation -> TraceOf Observation -> Prop :=
+| ObsPreTau1 : forall OO OO',
+    ObsTracePrefix OO OO' ->
+    ObsTracePrefix (notfinished Tau OO) OO'
+| ObsPreTau2 : forall OO OO',
+    ObsTracePrefix OO OO' ->
+    ObsTracePrefix OO (notfinished Tau OO')
+| ObsPreNow : forall w OO OO',
+    ObsTracePrefix OO OO' ->
+    ObsTracePrefix (notfinished (Out w) OO) (notfinished (Out w) OO')
+| ObsPreFinishedOut1 : forall w,
+    ObsTracePrefix (finished (Out w)) (finished (Out w))
+| ObsPreFinishedOut2 : forall w OO,
+    ObsTracePrefix (notfinished (Out w) OO) (finished (Out w))
+| ObsPreFinishedTau : forall OO,
+    ObsTracePrefix OO (finished Tau)
+| ObsPreAllTau : forall OO,
+     ObsTracePrefix OO OO.
+
+Notation "OO' <=_O OO" := (ObsTracePrefix OO OO') (at level 80).
+
+Definition ObsTracePrefApp' :
+  forall O1 O1' O2 O2' o1 o1',
+    Last O1 o1 -> Last O1' o1' -> 
+    ObsTraceEq O1 O1' ->
+    ObsTracePrefix O2 O2' ->
+    ObsTracePrefix (O1^(Some O2)) (O1'^(Some O2')).
+Proof.
+  intros O1 O1' O2 O2' o1 o1' H;
+    (* I really want SSR... *)
+    revert O1' O2 O2' o1'.
+  induction H as [o1|]; intros O1' O2 O2' o1' Last' Eq Pref.
+  - generalize dependent O2;
+    generalize dependent O2';
+    generalize dependent Eq.
+    induction Last';
+      intros Eq O2' O2 Pref.
+    + inversion Eq; subst; simpl in *; clear Eq; app_frobber.
+      (* Hint constructors doesn't work for this? *)
+      * apply ObsPreNow; auto.
+      * apply ObsPreTau1; apply ObsPreTau2; auto.
+      * destruct a.
+        -- apply ObsPreNow; auto.
+        -- apply ObsPreTau1; apply ObsPreTau2; auto.
+    + inversion Eq; subst; simpl in *; clear Eq.
+      specialize (IHLast' H1 O2' O2 Pref).      
+      app_frobber.
+      eapply ObsPreTau2.
+      auto.
+  (* Try by inversion. *)
+  - destruct a'.
+    + destruct (EqOut_tauN O1' o1' Last' w T Eq) as [n [HTau | [T' HTau]]].
+      * rewrite HTau in *.
+        clear HTau.
+        induction n; simpl in *; subst; app_frobber.
+        -- apply ObsPreNow.
+           inversion Eq. (* This makes me feel strange *)
+        -- apply ObsPreTau2.
+           inversion Last'; subst; clear Last'.
+           apply ObsTraceEqRemoveTau2 in Eq.
+           specialize (IHn H3 Eq).
+           auto.
+      * rewrite HTau in *.
+        clear HTau.
+        induction n; simpl in *; subst; app_frobber.
+        -- apply ObsPreNow.
+           inversion Eq; subst; clear Eq.
+           ++ inversion Last'; subst; clear Last'.
+              eauto.
+           ++ inversion Last'; subst; clear Last'.
+              eauto using ObsEqAllTau.
+        -- inversion Last'; subst; clear Last'.
+           specialize (IHn H3).
+           apply ObsTraceEqRemoveTau2 in Eq.
+           specialize (IHn Eq).
+           apply ObsPreTau2.
+           auto.
+    + apply ObsTraceEqRemoveTau1 in Eq.
+      app_frobber.
+      apply ObsPreTau1.
+      eauto.
+Qed.
